Hoare/HoareTripleForBasicBlocks.thy
@@ -1,0 +1,328 @@
+(*
+   Copyright 2017 Myriam Begel
+
+   Licensed under the Apache License, Version 2.0 (the "License");
+   you may not use this file except in compliance with the License.
+   You may obtain a copy of the License at
+
+       http://www.apache.org/licenses/LICENSE-2.0
+
+   Unless required by applicable law or agreed to in writing, software
+   distributed under the License is distributed on an "AS IS" BASIS,
+   WITHOUT WARRANTIES OR CONDITIONS OF ANY KIND, either express or implied.
+   See the License for the specific language governing permissions and
+   limitations under the License.
+*)
+
+theory "HoareTripleForBasicBlocks"
+
+imports "HoareTripleForInstructions"
+"../attic/BasicBlocks"
+"../EvmFacts"
+
+begin
+type_synonym pred = "(state_element set \<Rightarrow> bool)"
+
+(* We define here the program logic for BLOCKSs *)
+(* We start with Hoare triples valid for the execution of one instruction *)
+
+(* We have to add more instructions here *)
+definition iszero_stack :: "w256 \<Rightarrow> w256" where
+"iszero_stack w = (if w = 0 then (word_of_int 1) else (word_of_int 0))"
+
+fun arith_2_1_low:: "arith_inst \<Rightarrow> w256 \<Rightarrow> w256 \<Rightarrow> w256" where
+ "arith_2_1_low MUL = (\<lambda> a b .  a * b) "
+| "arith_2_1_low DIV =
+	(\<lambda> a divisor .
+		(if divisor =(((word_of_int 0) ::  256 word))
+			then(((word_of_int 0) ::  256 word))
+			else (\<lambda> i .  word_of_int ( i)) ((Word.uint a) div (Word.uint divisor))))"
+| "arith_2_1_low MOD =
+  (\<lambda> a divisor .  (if divisor =(((word_of_int 0) ::  256 word)) then(((word_of_int 0) ::  256 word)) else
+            (\<lambda> i .  word_of_int ( i)) ((Word.uint a) mod (Word.uint divisor))))"
+| "arith_2_1_low _ = (\<lambda> a b . 0)"
+
+fun arith_2_1_verylow:: "arith_inst \<Rightarrow> w256 \<Rightarrow> w256 \<Rightarrow> w256" where
+ "arith_2_1_verylow ADD = (\<lambda> a b .  a + b) "
+| "arith_2_1_verylow SUB = (\<lambda> a b .  a - b) "
+| "arith_2_1_verylow inst_GT =
+	(\<lambda> a b .  if a > b then(((word_of_int 1) ::  256 word)) else(((word_of_int 0) ::  256 word)))"
+| "arith_2_1_verylow inst_EQ =
+	(\<lambda> a b .  if a = b then(((word_of_int 1) ::  256 word)) else(((word_of_int 0) ::  256 word)))"
+| "arith_2_1_verylow inst_LT =
+	(\<lambda> a b .  if b > a then(((word_of_int 1) ::  256 word)) else(((word_of_int 0) ::  256 word)))"
+| "arith_2_1_verylow _ = (\<lambda> a b . 0)"
+
+fun arith_3_1:: "arith_inst \<Rightarrow> w256 \<Rightarrow> w256 \<Rightarrow> w256 \<Rightarrow> w256" where
+ "arith_3_1 ADDMOD =
+		(\<lambda> a b divisor .
+     (if divisor =(((word_of_int 0) ::  256 word)) then(((word_of_int 0) ::  256 word))
+			else (\<lambda> i .  word_of_int ( i)) ((Word.uint a + Word.uint b) mod (Word.uint divisor))))"
+| "arith_3_1 MULMOD =
+		(\<lambda> a b divisor .
+     (if divisor =(((word_of_int 0) ::  256 word)) then(((word_of_int 0) ::  256 word))
+			else (\<lambda> i .  word_of_int ( i)) ((Word.uint a * Word.uint b) mod (Word.uint divisor))))"
+| "arith_3_1 _ = (\<lambda> a b c . 0)"
+
+inductive triple_inst_arith :: "pred \<Rightarrow> pos_inst \<Rightarrow> pred \<Rightarrow> bool" where
+  inst_arith_2_1_low :
+    "i \<in> {MUL, DIV, MOD} \<Longrightarrow>
+		triple_inst_arith
+      (\<langle> h \<le> 1022 \<and> Glow \<le> g \<and> m \<ge> 0\<rangle> **
+       continuing \<and>* memory_usage m \<and>* program_counter n \<and>*
+       stack_height (Suc (Suc h)) \<and>* stack (Suc h) v \<and>* stack h w \<and>*
+			 gas_pred g \<and>* rest)
+      (n, Arith i)
+      (program_counter (n + 1) \<and>* continuing \<and>*
+       memory_usage m \<and>* stack_height (Suc h) \<and>*
+       stack h (arith_2_1_low i v w) \<and>*
+       gas_pred (g - Glow) \<and>* rest)"
+|  inst_arith_2_1_verylow :
+    "i \<in> {ADD, SUB, inst_GT, inst_EQ, inst_LT} \<Longrightarrow>
+		 triple_inst_arith
+      (\<langle> h \<le> 1022 \<and> Gverylow \<le> g \<and> m \<ge> 0\<rangle> **
+       continuing \<and>* memory_usage m \<and>* program_counter n \<and>*
+       stack_height (Suc (Suc h)) \<and>* stack (Suc h) v \<and>* stack h w \<and>*
+			 gas_pred g \<and>* rest)
+      (n, Arith i)
+      (program_counter (n + 1) \<and>* continuing \<and>*
+       memory_usage m \<and>* stack_height (Suc h) \<and>*
+       stack h (arith_2_1_verylow i v w) \<and>*
+       gas_pred (g - Gverylow) \<and>* rest)"
+|  inst_arith_3_1 :
+    "i \<in> {ADDMOD, MULMOD} \<Longrightarrow>
+		 triple_inst_arith
+      (\<langle> h \<le> 1021 \<and> Gmid \<le> g \<and> m \<ge> 0\<rangle> **
+       continuing \<and>* memory_usage m \<and>* program_counter n \<and>*
+       stack_height (Suc (Suc (Suc h))) \<and>* stack (Suc (Suc h)) u \<and>* stack (Suc h) v \<and>* stack h w \<and>*
+			 gas_pred g \<and>* rest)
+      (n, Arith i)
+      (program_counter (n + 1) \<and>* continuing \<and>*
+       memory_usage m \<and>* stack_height (Suc h) \<and>*
+       stack h (arith_3_1 i u v w) \<and>*
+       gas_pred (g - Gmid) \<and>* rest)"
+| inst_iszero :
+    "triple_inst_arith
+      (\<langle> h \<le> 1023 \<and> Gverylow \<le> g \<and> m \<ge> 0\<rangle> **
+       continuing \<and>* memory_usage m \<and>* program_counter n \<and>*
+       stack_height (Suc h) \<and>* stack h w \<and>* gas_pred g \<and>* rest)
+      (n, Arith ISZERO)
+      (program_counter (n + 1) \<and>* continuing \<and>*
+       memory_usage m \<and>* stack_height (Suc h) \<and>*
+       stack h (iszero_stack w) \<and>*
+       gas_pred (g - Gverylow) \<and>* rest)"
+
+fun bits_2_1_verylow:: "bits_inst \<Rightarrow> w256 \<Rightarrow> w256 \<Rightarrow> w256" where
+ "bits_2_1_verylow BYTE = get_byte"
+| "bits_2_1_verylow inst_AND = (\<lambda> a b .  a AND b)"
+| "bits_2_1_verylow inst_OR = (\<lambda> a b .  a OR b)"
+| "bits_2_1_verylow inst_XOR = (\<lambda> a b .  a XOR b)"
+| "bits_2_1_verylow _ = (\<lambda> a b  . 0)"
+
+inductive triple_inst_bits :: "pred \<Rightarrow> pos_inst \<Rightarrow> pred \<Rightarrow> bool" where
+  inst_instNOT :
+    "triple_inst_bits
+      (\<langle> h \<le> 1023 \<and> Gverylow \<le> g \<and> m \<ge> 0\<rangle> **
+       continuing \<and>* memory_usage m \<and>* program_counter n \<and>*
+       stack_height (Suc h) \<and>* stack h w \<and>* gas_pred g \<and>* rest)
+      (n, Bits inst_NOT)
+      (program_counter (n + 1) \<and>* continuing \<and>*
+       memory_usage m \<and>* stack_height (Suc h) \<and>*
+       stack h (NOT w) \<and>*
+       gas_pred (g - Gverylow) \<and>* rest)"
+|  inst_bits_2_1_verylow :
+    "i \<in> {inst_AND, inst_OR, inst_XOR, BYTE} \<Longrightarrow>
+		 triple_inst_bits
+      (\<langle> h \<le> 1022 \<and> Gverylow \<le> g \<and> m \<ge> 0\<rangle> **
+       continuing \<and>* memory_usage m \<and>* program_counter n \<and>*
+       stack_height (Suc (Suc h)) \<and>* stack (Suc h) v \<and>* stack h w \<and>*
+			 gas_pred g \<and>* rest)
+      (n, Bits i)
+      (program_counter (n + 1) \<and>* continuing \<and>*
+       memory_usage m \<and>* stack_height (Suc h) \<and>*
+       stack h (bits_2_1_verylow i v w) \<and>*
+       gas_pred (g - Gverylow) \<and>* rest)"
+
+inductive triple_inst_pc :: "pred \<Rightarrow> pos_inst \<Rightarrow> pred \<Rightarrow> bool" where
+  inst_jumpdest :
+    "triple_inst_pc
+      (\<langle> h \<le> 1024 \<and> Gjumpdest \<le> g \<and> m \<ge> 0\<rangle> \<and>*
+       continuing \<and>* memory_usage m \<and>* program_counter n \<and>*
+       stack_height h \<and>* gas_pred g \<and>* rest)
+      (n, Pc JUMPDEST)
+      (program_counter (n + 1) \<and>* continuing \<and>*
+       memory_usage m \<and>* stack_height h \<and>*
+       gas_pred (g - Gjumpdest) \<and>* rest)"
+| inst_pc :
+    "triple_inst_pc
+      (\<langle> h \<le> 1023 \<and> Gbase \<le> g \<and> m \<ge> 0\<rangle> **
+       continuing \<and>* memory_usage m \<and>* program_counter n \<and>*
+       stack_height h \<and>* gas_pred g \<and>* rest)
+      (n, Pc PC)
+      (program_counter (n + 1) \<and>* continuing \<and>*
+       memory_usage m \<and>* stack_height (Suc h) \<and>*
+       stack h (word_of_int n) \<and>*
+       gas_pred (g - Gbase) \<and>* rest)"
+
+inductive triple_inst_stack :: "pred \<Rightarrow> pos_inst \<Rightarrow> pred \<Rightarrow> bool" where
+  inst_push_n :
+    "triple_inst_stack
+      (\<langle> h \<le> 1023 \<and> length lst > 0 \<and> 32 \<ge> length lst \<and> Gverylow \<le> g \<and> m \<ge> 0\<rangle> \<and>*
+       continuing \<and>* program_counter n \<and>*
+       memory_usage m \<and>* stack_height h \<and>*
+       gas_pred g \<and>* rest)
+      (n, Stack (PUSH_N lst))
+      (program_counter (n + (1 + int (length lst))) \<and>*
+       continuing \<and>* memory_usage m \<and>*
+       stack_height (Suc h) \<and>* gas_pred (g - Gverylow) \<and>*
+       stack h (word_rcat lst) \<and>* rest)"
+| inst_pop :
+    "triple_inst_stack
+      (\<langle> h \<le> 1023 \<and> Gbase \<le> g \<and> m \<ge> 0\<rangle> **
+       continuing \<and>* memory_usage m \<and>* program_counter n \<and>*
+       stack_height (Suc h) \<and>* stack h w \<and>* gas_pred g \<and>* rest)
+      (n, Stack POP)
+      (program_counter (n + 1) \<and>* continuing \<and>*
+       memory_usage m \<and>* stack_height h \<and>*
+       gas_pred (g - Gbase) \<and>* rest)"
+
+inductive triple_inst_misc :: "pred \<Rightarrow> pos_inst \<Rightarrow> pred \<Rightarrow> bool" where
+ inst_stop :
+    "triple_inst_misc
+      (\<langle> h \<le> 1024 \<and> 0 \<le> g \<and> m \<ge> 0\<rangle> \<and>* continuing \<and>* memory_usage m \<and>*
+       program_counter n \<and>* stack_height h \<and>* gas_pred g \<and>* rest)
+      (n, Misc STOP)
+      (stack_height h \<and>* not_continuing \<and>* memory_usage m \<and>*
+       program_counter n \<and>* action (ContractReturn []) \<and>*
+       gas_pred g \<and>* rest)"
+
+inductive triple_inst :: "pred \<Rightarrow> pos_inst \<Rightarrow> pred \<Rightarrow> bool" where
+  inst_arith :
+    "triple_inst_arith p (n, Arith i) q \<Longrightarrow> triple_inst p (n, Arith i) q"
+| inst_bits :
+    "triple_inst_bits p (n, Bits i) q \<Longrightarrow> triple_inst p (n, Bits i) q"
+| inst_misc :
+    "triple_inst_misc p (n, Misc i) q \<Longrightarrow> triple_inst p (n, Misc i) q"
+| inst_pc :
+    "triple_inst_pc p (n, Pc i) q \<Longrightarrow> triple_inst p (n, Pc i) q"
+| inst_stack :
+    "triple_inst_stack p (n, Stack i) q \<Longrightarrow> triple_inst p (n, Stack i) q"
+| inst_swap :
+		"triple_inst
+			(\<langle> h \<le> 1024 \<and> Suc (unat n) < h \<and> g \<ge> Gverylow \<and> m \<ge> 0\<rangle> **
+			 stack_height h ** stack (h - 1) w ** stack (h - (unat n) - 2) v **
+			 program_counter k ** gas_pred g ** memory_usage m **
+			 continuing ** rest)
+			(k, Swap n)
+			(program_counter (k + 1) ** gas_pred (g - Gverylow) **
+			 stack_height h ** stack (h - 1) v ** stack (h - (unat n) - 2) w **
+			 memory_usage m ** continuing ** rest)"
+| inst_strengthen_pre:
+    "triple_inst p i q \<Longrightarrow> (\<And>s. r s \<Longrightarrow> p s) \<Longrightarrow> triple_inst r i q"
+| inst_false_pre:
+    "triple_inst \<langle>False\<rangle> i post"
+
+(* We define here the program logic for BLOCKSs *)
+(* We start with Hoare triples valid for the execution of one instruction *)
+
+inductive triple_seq :: "pred \<Rightarrow> pos_inst list \<Rightarrow> pred \<Rightarrow> bool" where
+  seq_inst :
+  "\<lbrakk>triple_inst pre x q;
+    triple_seq q xs post \<rbrakk> \<Longrightarrow>
+   triple_seq pre (x#xs) post"
+| seq_empty:
+  "(\<And>s. pre s \<Longrightarrow> post s) \<Longrightarrow>
+   triple_seq pre [] post"
+| seq_strengthen_pre:
+  "triple_seq p xs q \<Longrightarrow>
+   (\<And>s. r s \<Longrightarrow> p s) \<Longrightarrow>
+   triple_seq r xs q"
+| seq_false_pre:
+  "triple_seq \<langle>False\<rangle> xs post"
+
+inductive triple_blocks :: "basic_blocks \<Rightarrow> pred \<Rightarrow> vertex \<Rightarrow> pred \<Rightarrow> bool" where
+  blocks_no :
+  "triple_seq pre insts post \<Longrightarrow>
+   triple_blocks blocks pre (n, insts, No) post"
+| blocks_next :
+  "\<lbrakk>triple_seq pre insts (program_counter i \<and>* q);
+    i = n + inst_size_list insts;
+    blocks_list blocks i = Some (bi, ti);
+    triple_blocks blocks (program_counter i \<and>* q) (i, bi, ti) post\<rbrakk> \<Longrightarrow>
+   triple_blocks blocks pre (n, insts, Next) post"
+| blocks_jump :
+  "\<lbrakk>triple_seq pre insts
+      (\<langle> h \<le> 1023 \<and> Gmid \<le> g \<and> m \<ge> 0\<rangle> \<and>*
+       program_counter (n + inst_size_list insts) \<and>* gas_pred g \<and>*
+       memory_usage m \<and>* stack_height (Suc h) \<and>*
+       stack h (word_of_int dest::256 word) \<and>*
+       continuing \<and>* rest);
+    blocks_list blocks dest = Some (bi, ti);
+    bi = (dest, Pc JUMPDEST) # bbi;
+    triple_blocks blocks
+      (program_counter dest \<and>* gas_pred (g - Gmid) \<and>*
+       memory_usage m \<and>* stack_height h \<and>*
+       continuing \<and>* rest)
+      (dest, bi, ti) post\<rbrakk> \<Longrightarrow>
+   triple_blocks blocks pre (n, insts, Jump) post"
+| blocks_jumpi :
+  "\<lbrakk>  triple_seq pre insts
+      ((\<langle> h \<le> 1022  \<and> Ghigh \<le> g \<and> m \<ge> 0\<rangle> \<and>*
+       stack_height (Suc (Suc h)) \<and>*
+       stack (Suc h) (word_of_int dest::256 word) \<and>*
+       stack h cond \<and>* gas_pred g \<and>*
+       continuing \<and>* memory_usage m \<and>*
+       program_counter (n + inst_size_list insts) \<and>* rest));
+    j = n + 1 + inst_size_list insts;
+    blocks_list blocks dest = Some (bi, ti);
+    bi = (dest, Pc JUMPDEST) # bbi;
+    blocks_list blocks j = Some (bj, tj);
+    r = (stack_height h \<and>* gas_pred (g - Ghigh) \<and>*
+         continuing \<and>* memory_usage m \<and>* rest);
+    (cond \<noteq> 0 \<Longrightarrow> triple_blocks blocks (r \<and>* program_counter dest) (dest, bi, ti) post);
+    (cond = 0 \<Longrightarrow> triple_blocks blocks (r \<and>* program_counter j) (j, bj, tj) post)\<rbrakk> \<Longrightarrow>
+   triple_blocks blocks pre (n, insts, Jumpi) post"
+| blocks_false_pre:
+  "triple_blocks blocks \<langle>False\<rangle> i post"
+
+lemma blocks_jumpi_uint:
+"\<lbrakk>  triple_seq pre insts
+      ((\<langle> h \<le> 1022  \<and> Ghigh \<le> g \<and> m \<ge> 0\<rangle> \<and>*
+       stack_height (Suc (Suc h)) \<and>*
+       stack (Suc h) dest \<and>*
+       stack h cond \<and>* gas_pred g \<and>*
+       continuing \<and>* memory_usage m \<and>*
+       program_counter (n + inst_size_list insts) \<and>* rest));
+    j = n + 1 + inst_size_list insts;
+    blocks_list blocks (uint dest) = Some (bi, ti);
+    bi = (uint dest, Pc JUMPDEST) # bbi;
+    blocks_list blocks j = Some (bj, tj);
+    r = (stack_height h \<and>* gas_pred (g - Ghigh) \<and>*
+         continuing \<and>* memory_usage m \<and>* rest);
+    (cond \<noteq> 0 \<Longrightarrow> triple_blocks blocks (r \<and>* program_counter (uint dest)) (uint dest, bi, ti) post);
+    (cond = 0 \<Longrightarrow> triple_blocks blocks (r \<and>* program_counter j) (j, bj, tj) post)\<rbrakk> \<Longrightarrow>
+   triple_blocks blocks pre (n, insts, Jumpi) post"
+apply(rule blocks_jumpi)
+defer
+apply(assumption)+
+apply(simp)
+done
+
+lemma blocks_jump_uint :
+  "\<lbrakk>triple_seq pre insts
+      (\<langle> h \<le> 1023 \<and> Gmid \<le> g \<and> m \<ge> 0\<rangle> \<and>*
+       program_counter (n + inst_size_list insts) \<and>* gas_pred g \<and>*
+       memory_usage m \<and>* stack_height (Suc h) \<and>*
+       stack h dest \<and>*
+       continuing \<and>* rest);
+    blocks_list blocks (uint dest) = Some (bi, ti);
+    bi = (uint dest, Pc JUMPDEST) # bbi;
+    triple_blocks blocks
+      (program_counter (uint dest) \<and>* gas_pred (g - Gmid) \<and>*
+       memory_usage m \<and>* stack_height h \<and>*
+       continuing \<and>* rest)
+      (uint dest, bi, ti) post\<rbrakk> \<Longrightarrow>
+   triple_blocks blocks pre (n, insts, Jump) post"
+by(rule blocks_jump; simp)
+
+end
